code/ecdsap256/Hacl.P256.fst
@@ -83,3 +83,6 @@ let is_more_than_zero_less_than_order x =
   Hacl.Impl.P256.Signature.Common.isMoreThanZeroLessThanOrder x
 
 let ecp256scalar_mult result pubKey scalar = Hacl.Impl.P256.ScalarMult.ecp256scalar_mult result pubKey scalar
+
+
+let point_add8 result p q = Hacl.Impl.P256.PointAdd8.point_add8 result p q
