code/ecdsap256/Hacl.P256.fsti
@@ -425,3 +425,35 @@ val ecp256scalar_mult:
       modifies (loc result) h0 h1 /\
       as_seq h1 (gsub result (size 0) (size 32)) == pointX /\
       as_seq h1 (gsub result (size 32) (size 32)) == pointY)
+
+
+[@ (Comment "
+  \n Input: result: uint8[64], \n point p: uint8[64], \n point q: uint8[64].
+  \n Output: void, result = P + Q
+  ")]
+val point_add8: result: lbuffer uint8 (size 64) -> p: lbuffer uint8 (size 64) -> q: lbuffer uint8 (size 64) -> 
+  Stack unit 
+  (requires fun h -> live h result /\ live h p /\ live h q /\ (
+    let pX = gsub p (size 0) (size 32) in 
+    let pY = gsub p (size 32) (size 32) in 
+    let qX = gsub q (size 0) (size 32) in 
+    let qY = gsub q (size 32) (size 32) in
+    
+    Lib.ByteSequence.nat_from_bytes_be (as_seq h pX) < prime256 /\ 
+    Lib.ByteSequence.nat_from_bytes_be (as_seq h pY) < prime256 /\
+    Lib.ByteSequence.nat_from_bytes_be (as_seq h qX) < prime256 /\
+    Lib.ByteSequence.nat_from_bytes_be (as_seq h qY) < prime256))
+  (ensures fun h0 _ h1 -> modifies (loc result) h0 h1 /\ (
+    let open Lib.ByteSequence in 
+    let pX = nat_from_bytes_be (as_seq h0 (gsub p (size 0) (size 32))) in 
+    let pY = nat_from_bytes_be (as_seq h0 (gsub p (size 32) (size 32))) in
+    let pK = Spec.P256.toJacobianCoordinates (pX, pY) in 
+    
+    let qX = nat_from_bytes_be (as_seq h0 (gsub q (size 0) (size 32))) in 
+    let qY = nat_from_bytes_be (as_seq h0 (gsub q (size 32) (size 32))) in
+    let qK = Spec.P256.toJacobianCoordinates (qX, qY) in 
+    let resultX, resultY, _ = Spec.P256._norm (Spec.P256._point_add pK qK) in 
+    
+    as_seq h1 (gsub result (size 0) (size 32)) == nat_to_bytes_be 32 resultX /\
+    as_seq h1 (gsub result (size 32) (size 32)) == nat_to_bytes_be 32 resultY))
+
